src/list.h
@@ -1,3 +1,9 @@
+/*  Titre:      src/list.h
+    Auteur:     Adrien Stalain
+
+    Fait dans le cadre d'un stage à Orange Labs
+*/
+
 #ifndef LIST_H
 #define LIST_H
 
@@ -22,5 +28,13 @@ void list_insert_after(struct list *node, struct list *new);
 struct list *list_find_last_node(list_t *l);
 
 void list_insert_back(list_t *l, struct list *new);
+
+struct list *list_pop(list_t *l);
+
+unsigned int list_length(list_t *l);
+
+int list_is_empty(list_t *l);
+
+void list_reverse(list_t *l);
 
 #endif
