proof/Import_C.thy
@@ -1,3 +1,9 @@
+(*  Titre:      Import_C.thy
+    Auteur:     Adrien Stalain
+
+    Fait dans le cadre d'un stage à Orange Labs
+*)
+
 theory Import_C
   imports "AutoCorres.AutoCorres"
 begin
